going well, but bloody bumps appearing ahead again

system-f/Syntax.v
@@ -1,6 +1,7 @@
 (** This file defines the syntax of System F.  Based on Filip’s development of System T. (github.com/finrod) *)
 
- 
+Require Import ZArith.
+
 (* Types *)
 Inductive ty :=
 | tvar    : nat -> ty
@@ -11,6 +12,7 @@ Notation " ## n " := (tvar n) (at level 20) : t_scope.
 Notation " A 'arrows' B " := (tarrow A B) (at level 30, right associativity) : t_scope.
 Notation "'allX' , A " := (tforall A) (at level 50) : t_scope.
 Open Scope t_scope.
+Open Scope list_scope.
 
 (* Terms *)
 (* The formalisation uses de Bruijn indices to deal with binders. *)
@@ -27,6 +29,8 @@ Notation " t * s " := (appl t s) (at level 40, left associativity) : t_scope.
 Notation "'ΛX' , t" := (Lam t) (at level 50) : t_scope.
 Notation " t @ A " := (inst t A) (at level 40, left associativity) : t_scope.
 
+Section Properties.
+
 Fixpoint closed (n:nat) (t:tm) : Prop :=
 match t with 
   | #k => k < n
@@ -35,5 +39,23 @@ match t with
   | ΛX, t' => closed n t'
   | s @ A => closed n s
 end.
+
+Fixpoint closed_list (γ:list tm) : Prop :=
+match γ with
+  | nil => True
+  | t :: γ' => (closed 0 t) /\ (closed_list γ')
+end.
+
+Lemma closed_monotone t : forall j k, j <= k -> closed j t -> closed k t.
+  induction t as [ n | A t0 IH | t0 IH0 t1 IH1 | t0 IH | t0 IH A]; intros; 
+    simpl in *.
+      omega.
+      apply IH with (S j); try omega; assumption.  
+      split.  apply IH0 with j; tauto.  apply IH1 with j; tauto. 
+      apply IH with j; tauto.
+      apply IH with j; tauto.
+Qed.
+
+End Properties.
 
 Close Scope t_scope.
